CellularAutomatas/proofs/two_stage_is_rt_closed.lean
@@ -26,102 +26,81 @@ open FiniteStateTransducer (M_map M_prod M_projQ M_id)
 open CellAutomaton
 
 
-def prefix_mem (L: Language α) [DecidablePred L] (w: Word α): Word Bool :=
-  (List.range w.length).map (fun i => decide (L (w⟦0..i+1⟧)))
-
-@[simp]
-lemma prefix_mem_len {α} (L: Language α) [DecidablePred L] (w: Word α):
-  (prefix_mem L w).length = w.length := by
-  simp [prefix_mem]
-
-def prefix_mem_adv (L: Language α) [DecidablePred L]: Advice α Bool := { f := prefix_mem L }
-
-def lift {α β} [Alphabet α] [Alphabet β]
-    (f: Word α → Word β) (L: Language α): Language β :=
-  { w: Word β | ∃ v: Word α, f v = w ∧ L v }
-
-
-
-
-
-
-
-
-
-
 variable {α: Type} [Alphabet α]
 variable {Γ: Type} [Alphabet Γ]
 
-def CA_rt_to_TwoStage (C: CA_rt α): TwoStageAdvice α Bool :=
+
+section CountUntil
+
+def some_fin (k: ℕ) (i: ℕ): Option (Fin k) :=
+  if h: i < k then
+    some (Fin.mk i (by simp [h]))
+  else
+    none
+
+lemma some_fin_succ: ((some_fin k v) >>= fun v => some_fin k (v + 1)) = some_fin k (v + 1) := by
+  unfold some_fin
+  grind
+
+def c_count_until {α} [Alphabet α] (k: ℕ) [NeZero k]: CellAutomaton α (Fin k)？ :=
   {
-    β := Bool
-    C := C.val.toCellAutomaton
-    M := FiniteStateTransducer.M_id Bool
+    Q := (Fin k)？
+    δ := fun _ q2 _ => q2 >>= fun v => some_fin k (v.val + 1)
+    embed := fun _ => some 0
+    project := id
   }
 
-lemma CA_rt_to_TwoStage_advice_eq (C: CA_rt α) :
-  (CA_rt_to_TwoStage C).advice.f = C.val.trace_rt := by
-  funext w
-  simp [CA_rt_to_TwoStage, TwoStageAdvice.advice]
+@[simp]
+lemma c_count_until_spec_config {α} [Alphabet α] (k: ℕ) [h: NeZero k] (c: Config α):
+    (c_count_until k).comp (embed_config c) t i = some_fin k t := by
+  rw [comp_config_eq_project_nextt]
+  change ((c_count_until k).nextt ⦋c⦌ t) i = some_fin k t
 
-lemma CA_rt_to_TwoStage_eq (C: CA_rt α):
-  (CA_rt_to_TwoStage C).advice.f = (Advice.prefixes_in_L C.val.L).f := by
-  rw [CA_rt_to_TwoStage_advice_eq]
-  funext w
-  apply List.ext_getElem
-  · simp
-  · intro i h1 h2
-    have (v: Bool) (p: Prop) [Decidable p]: (v = decide p ↔ (v = true ↔ p)) := by grind
-    simp [Advice.prefixes_in_L, this, trace_rt_getElem_i_iff]
-    rfl
+  induction t generalizing i with
+  | zero =>
+    simp [c_count_until, embed_config, some_fin, h.out]
+  | succ t ih =>
+    rw [nextt_succ]
+    simp [CellAutomaton.next]
+    simp [ih]
+    simp [c_count_until]
+    exact some_fin_succ
 
+@[simp]
+def c_count_until_spec_word {α} [Alphabet α] (k: Nat) [NeZero k] (w: Word α):
+    (c_count_until k).comp (embed_word w) t i = some_fin k t := by
+  rw [embed_word]
+  rw [c_count_until_spec_config]
 
-theorem advice_prefixes_in_L_is_two_stage_advice (C: CA_rt α):
-    (Advice.prefixes_in_L C.val.L).is_two_stage_advice := by
-  use CA_rt_to_TwoStage C
-  have h_eq := CA_rt_to_TwoStage_eq C
-  match (CA_rt_to_TwoStage C).advice, (Advice.prefixes_in_L C.val.L), h_eq with
-  | ⟨f1, l1⟩, ⟨f2, l2⟩, h =>
-    simp at h
-    subst h
-    rfl
+end CountUntil
 
 
 
-noncomputable def get_ca (L: ℒ (CA_rt α)): CA_rt α := by
-  have := L.prop
-  rw [ℒ_CA_rt_iff] at this
-  exact ⟨ Classical.choose this, by simp [Classical.choose_spec this] ⟩
+
+@[simp]
+lemma word_to_config_empty {α} [Alphabet α] :
+    word_to_config (α := α) [] = fun _ => none := by
+  funext i
+  simp [word_to_config]
+
+@[simp]
+lemma embed_word_p_not_in_range {α} [Alphabet α] (w: Word α) {C: CellAutomaton α？ β} (p: ℤ) (h: p ∉ w.range):
+    (embed_word (C := C) w) p = C.embed none := by
+  unfold embed_word word_to_config embed_config
+  have :  ¬ (0 ≤ p ∧ p < ↑(List.length w)) := by grind [Word.range]
+  simp [this]
 
 
-noncomputable def prefix_mem_two_stage (L: ℒ (CA_rt α)): TwoStageAdvice α Bool :=
-  CA_rt_to_TwoStage (get_ca L)
-
-def prefix_mem_two_stage_spec (L: ℒ (CA_rt α)) [DecidablePred L.val]:
-    (prefix_mem_two_stage L).advice.f = prefix_mem L.val := by
-  sorry
-
-lemma advice_eq_iff {α β: Type} (adv1 adv2: Advice α β) (h: adv1.f = adv2.f): adv1 = adv2 := by
-  cases adv1
-  cases adv2
-  simp at h
-  subst h
-  rfl
+@[simp]
+lemma embed_word_p_in_range {α} [Alphabet α] (w: Word α) {C: CellAutomaton α？ β} (p: ℤ) (h: p ∈ w.range):
+    (embed_word (C := C) w) p = C.embed (w[p.toNat]'(by grind [Word.range])) := by
+  unfold embed_word word_to_config embed_config
+  have :  (0 ≤ p ∧ p < ↑(List.length w)) := by grind [Word.range]
+  simp [this]
 
 
-lemma L_rt_iff_prefix_mem_two_stage (L: Language α) [DecidablePred L]:
-    L ∈ ℒ (CA_rt α) ↔ (prefix_mem_adv L).is_two_stage_advice := by
-  constructor
-  · intro h
-    use prefix_mem_two_stage (⟨L, h⟩ : ℒ (CA_rt α))
-    apply advice_eq_iff
-    simp [prefix_mem_adv, prefix_mem_two_stage_spec]
-  · intro h
-    rw [ℒ_CA_rt_iff]
-    sorry
 
 
--- classical
 
 def ca_to_two_stage (C: CArtTransducer α Γ): TwoStageAdvice α Γ :=
   {
@@ -130,6 +109,15 @@ def ca_to_two_stage (C: CArtTransducer α Γ): TwoStageAdvice α Γ :=
     M := FiniteStateTransducer.M_id Γ
   }
 
+@[simp]
+lemma ca_to_two_stage_spec (C: CArtTransducer α Γ):
+    (ca_to_two_stage C).advice.f = C.trace_rt := by
+  funext w
+  simp [ca_to_two_stage, TwoStageAdvice.advice]
+
+
+
+
 
 def zip_two_stage [Alphabet α] [Alphabet β] [Alphabet γ] (a1: TwoStageAdvice α β) (a2: TwoStageAdvice α γ):
     TwoStageAdvice α (β × γ) :=
@@ -137,40 +125,213 @@ def zip_two_stage [Alphabet α] [Alphabet β] [Alphabet γ] (a1: TwoStageAdvice 
   let fst_new := a1.M ⨂ a2.M
   TwoStageAdvice.from_transducers fst_new ca_new
 
+@[simp]
+def zip_spec [Alphabet α] [Alphabet β] [Alphabet γ] (a1: TwoStageAdvice α β) (a2: TwoStageAdvice α γ):
+    (zip_two_stage a1 a2).advice.f w = (a1.advice.f w ⨂ a2.advice.f w) := by
+  simp [zip_two_stage, TwoStageAdvice.advice, TwoStageAdvice.from_transducers]
+  rfl
+
 infixl:65 " ⨂ " => zip_two_stage
 
-noncomputable def A (adv: TwoStageAdvice α Γ) (L: Language α): TwoStageAdvice α Bool :=
-  (prefix_mem_two_stage ⟨(lift adv.advice.annotate L), sorry⟩) ⊚ ((ca_to_two_stage (ca_id_word α)) ⨂ adv)
 
-lemma A_spec (adv: TwoStageAdvice α Γ) (L: Language α) [DecidablePred L]:
-    (A adv L).advice = prefix_mem_adv L := by
-  apply advice_eq_iff
-  funext w
-  simp [A, TwoStageAdvice.advice]
-  sorry
 
-lemma rt_closed_iff (adv: Advice α Γ):
-    adv.rt_closed ↔ (∀ L, (lift adv.annotate L) ∈ ℒ (CA_rt (α × Γ)) → L ∈ ℒ (CA_rt α)) := by
 
+
+
+
+
+lemma embed_word_p_eq {α} [Alphabet α] (w: Word α) {C: CellAutomaton α？ β} (p: ℤ):
+    (embed_word (C := C) w) p = C.embed (if h: p ≥ 0 ∧ p < w.length then w[p.toNat] else none) := by
+  unfold embed_word word_to_config embed_config
+  grind
+
+
+section CisBorder
+
+def c_is_border (α) [Alphabet α]: CellAutomaton α？ Bool :=
+  {
+    Q := Bool
+    δ := fun _ val _ => val
+    embed
+    | none => true
+    | some _ => false
+    project := id
+  }
+
+@[simp]
+lemma c_is_border_spec {α} [Alphabet α] (w: Word α):
+    (c_is_border α).comp w t 0 = (w == []) := by
+  unfold comp
+  erw [Function.id_comp]
+
+  induction t with
+  | zero =>
+    rw [nextt_zero]
+    rw [embed_word_p_eq]
+    unfold c_is_border
+    cases w
+    · simp
+    · simp
+  | succ t ih =>
+    rw [nextt_succ]
+    unfold CellAutomaton.next
+    rw [ih]
+    simp [c_is_border]
+
+end CisBorder
+
+
+
+section fix_empty
+
+variable {α: Type} [Alphabet α]
+
+
+def fix_empty (contains_empty: Bool) (C: CA_rt α): CA_rt α :=
+    toRtCa ((C.val.toCellAutomaton ⨂ c_is_border α).map_project (fun (a, b) => if b then contains_empty else a))
+
+@[simp]
+lemma fix_empty_spec (contains_empty: Bool) (C: CA_rt α)  (w: Word α):
+    w ∈ (fix_empty contains_empty C).val.L ↔ if w == [] then contains_empty else w ∈ C.val.L := by
+  rw [CA_rt_L_iff]
+  unfold embed_word
+  erw [map_project_comp]
+  rw [ca_zip_comp]
+  simp [CA_rt_L_iff]
+
+end fix_empty
+
+
+
+
+
+
+
+
+lemma subset_iff {α} {A B: Set α}: A ⊆ B ↔ (∀ L, L ∈ A → L ∈ B) := by rfl
+
+
+lemma advice_rt_closed_iff (adv: Advice α Γ):
+    adv.rt_closed ↔ (∀ (C : CA_rt (α ⨉ Γ)), {w | w ⨂ adv.f w ∈ C.val.L} ∈ ℒ (CA_rt α)) := by
   unfold Advice.rt_closed
-  unfold adviceAdd
-  conv in (ℒ (CA_rt (α ⨉ Γ) + adv) ) =>
-    change L ∈ tCellAutomatonWithAdvice.with_advice (CA_rt (α × Γ)) adv
+  rw [subset_antisymm_iff]
+  simp only [CA_rt_subseteq_CA_rt_with_advice adv, and_true]
+  rw [subset_iff]
+  simp [ℒ_oca_def]
+  grind
 
-  sorry
+lemma tCellAutomatonWithAdvice.L_mem_ℒ (C: CA_rt (α × Γ)) (adv: Advice α Γ): (C.val + adv).L ∈ ℒ (CA_rt (α ⨉ Γ) + adv) := by
+  unfold ℒ
+  simp only [HAdd.hAdd, Set.mem_setOf_eq, DefinesLanguage.L, exists_exists_and_eq_and]
+  use C
+  simp
+
+lemma tCellAutomatonWithAdvice.exists_CA_rt_of_rt_closed {adv: Advice α Γ} (h: adv.rt_closed) (C: CA_rt (α ⨉ Γ)):
+    ∃ (C' : CA_rt α), C'.val.L = (C.val + adv).L := by
+  have : (C.val + adv).L ∈ ℒ (CA_rt α) := by
+    unfold Advice.rt_closed at h
+    rw [←h]
+    exact tCellAutomatonWithAdvice.L_mem_ℒ C adv
+
+  rw [ℒ_CA_rt_iff] at this
+  simp [this]
+
+
+
+-- todo can be defined for any advice
+def TwoStageAdvice.L {α} [Alphabet α] (adv: TwoStageAdvice α Bool): Language α :=
+  { w: Word α | (adv.advice.f w).getLast? = true }
+
+
+def TwoStageAdvice.to_CA_rt {α} [Alphabet α] (adv: TwoStageAdvice α Bool): CA_rt α :=
+  fix_empty false (toRtCa $ adv.C.map_project (fun q => adv.M.f (adv.M.δ adv.M.q0 q)))
+
+
+
+@[simp]
+lemma TwoStageAdvice.to_CA_rt_L {α} [Alphabet α] (adv: TwoStageAdvice α Bool):
+    adv.to_CA_rt.val.L = adv.L := by
+  ext w
+
+  unfold TwoStageAdvice.to_CA_rt
+
+  by_cases h: w = []
+  · unfold TwoStageAdvice.L
+    rw [prop_of_elem_prop_set]
+    simp [h]
+
+  unfold TwoStageAdvice.L
+  rw [prop_of_elem_prop_set]
+
+  simp [h]
+  rw [←trace_rt_L h]
+  unfold TwoStageAdvice.advice
+  simp
+
+  erw [←FiniteStateTransducer.getLast?_of_scanr]
+  grind
+
+
+
+
+def TwoStageAdvice.from_CA_rt {α} [Alphabet α] (C: CA_rt α): TwoStageAdvice α Bool :=
+  {
+    β := Bool
+    C := C.val.toCellAutomaton
+    M := FiniteStateTransducer.M_id Bool
+  }
+
+@[simp]
+lemma TwoStageAdvice.from_CA_rt_spec {α} [Alphabet α] (C: CA_rt α):
+    (TwoStageAdvice.from_CA_rt C).advice.f = C.val.trace_rt := by
+  funext w
+  simp [TwoStageAdvice.from_CA_rt, TwoStageAdvice.advice]
+
+
+@[simp]
+lemma zip_left_empty {α} {v: Word β}: ([]: Word α) ⨂ v = [] := by simp [zip_words]
+
+@[simp]
+lemma zip_right_empty {α} {v: Word β}: v ⨂ ([]: Word α) = [] := by simp [zip_words]
+
+@[simp]
+lemma zip_empty_iff {α β} {v1: Word α} {v2: Word β}:
+    v1 ⨂ v2 = [] ↔ v1 = [] ∨ v2 = [] := by simp [zip_words]
+
 
 
 theorem two_stage_rt_closed (adv: TwoStageAdvice α Γ):
     adv.advice.rt_closed := by
-  open Classical in -- I'm quite sure this is not needed
+  open Classical in -- I'm quite sure this is not needed logically
 
-  suffices ∀ (L : Language α) (h: lift adv.advice.annotate L ∈ ℒ (CA_rt (α ⨉ Γ))), L ∈ ℒ (CA_rt α) from by
-    simp_all [rt_closed_iff]
+  rw [advice_rt_closed_iff]
+  intro C
+  rw [ℒ_CA_rt_iff]
 
-  intro L h
+  let x := ((TwoStageAdvice.from_CA_rt C) ⊚ ((ca_to_two_stage (ca_id_word α)) ⨂ adv))
+  let C' := fix_empty ([] ∈ C.val.L) x.to_CA_rt
 
-  suffices ∃ ts_adv: TwoStageAdvice α Bool, ts_adv.advice = prefix_mem_adv L from by
-    simp_all [L_rt_iff_prefix_mem_two_stage, Advice.is_two_stage_advice]
+  use C'
 
-  use A adv L
-  simp [A_spec adv]
+  constructor
+  · simp [C']
+
+  ext w
+
+
+  simp [C']
+  rw [prop_of_elem_prop_set]
+
+  by_cases h_empty: w = []
+  · simp [h_empty]
+
+  simp [h_empty]
+  simp [x]
+
+  unfold TwoStageAdvice.L
+  rw [prop_of_elem_prop_set]
+
+  have : ↑C ∈ CA_rt (α ⨉ Γ) := by simp
+  rw [elemL_iff_trace_rt this]
+
+  simp [h_empty]
