CellularAutomatas/proofs/advice_prefix_mem_rt_closed.lean
@@ -1,0 +1,44 @@
+import Mathlib.Data.Set.Basic
+import Mathlib.Data.Nat.Basic
+import Mathlib.Data.Nat.Find
+import Mathlib.Data.Fintype.Basic
+import Mathlib.Computability.Language
+import Mathlib.Data.Set.Lattice
+import Mathlib.Data.Nat.Lattice
+import Mathlib.Data.Fintype.Prod
+import CellularAutomatas.defs
+import CellularAutomatas.proofs.finite_state_transducers
+import CellularAutomatas.proofs.basic
+
+namespace CellularAutomatas
+
+variable {α: Type} [Alphabet α]
+
+def ts_prefix_mem (C: CA_rt α): TwoStageAdvice α Bool :=
+  {
+    β := Bool
+    C := C.val.toCellAutomaton
+    M := FiniteStateTransducer.M_id Bool
+  }
+
+
+lemma ts_prefix_mem_spec (C: CA_rt α): (ts_prefix_mem C).advice = Advice.prefix_mem C.val.L := by
+  apply advice_eq_iff
+  funext w
+
+  suffices C.val.trace_rt w = (Advice.prefix_mem C.val.L).f w by
+    unfold TwoStageAdvice.advice
+    simp only [ts_prefix_mem, FiniteStateTransducer.M_id_scanr_eq, Function.comp_apply, id_eq, this]
+
+  apply List.ext_getElem
+  · simp
+  · intro i h1 h2
+    have (v: Bool) (p: Prop) [Decidable p]: (v = decide p ↔ (v = true ↔ p)) := by grind
+    simp [Advice.prefix_mem, this, trace_rt_getElem_i_iff]
+    rfl
+
+
+theorem advice_prefix_mem_is_two_stage_advice (C: CA_rt α):
+    (Advice.prefix_mem C.val.L).is_two_stage_advice := by
+  use ts_prefix_mem C
+  simp [ts_prefix_mem_spec]
